proof/refine/RISCV64/Finalise_R.thy
@@ -2353,10 +2353,10 @@ lemma unbindNotification_invs[wp]:
     apply (auto split: if_split_asm)[1]
    apply (auto simp: tcb_st_not_Bound ntfn_q_refs_of'_mult split: if_split_asm)[1]
   apply (frule obj_at_valid_objs', clarsimp+)
-  apply (simp add: valid_ntfn'_def valid_obj'_def
+  apply (simp add: valid_ntfn'_def valid_obj'_def live'_def
             split: ntfn.splits)
   apply (erule if_live_then_nonz_capE')
-  apply (clarsimp simp: obj_at'_def ko_wp_at'_def)
+  apply (clarsimp simp: obj_at'_def ko_wp_at'_def live'_def)
   done
 
 lemma ntfn_bound_tcb_at':
@@ -2388,7 +2388,7 @@ lemma unbindMaybeNotification_invs[wp]:
            apply (fold_subgoals (prefix))[8]
            subgoal premises prems using prems
               by (auto simp: pred_tcb_at' valid_pspace'_def valid_obj'_def valid_ntfn'_def
-                             ko_wp_at'_def
+                             ko_wp_at'_def live'_def
                       elim!: obj_atE' if_live_then_nonz_capE'
                       split: option.splits ntfn.splits)
    apply (rule delta_sym_refs, assumption)
@@ -2789,7 +2789,7 @@ lemma tcbQueueRemove_tcbSchedNext_tcbSchedPrev_None_obj_at':
   apply (wpsimp wp: threadSet_wp getTCB_wp)
   by (fastforce dest!: heap_ls_last_None
                  simp: list_queue_relation_def prev_queue_head_def queue_end_valid_def
-                       obj_at'_def opt_map_def ps_clear_def objBits_simps
+                       obj_at'_def opt_map_def ps_clear_def gen_objBits_simps
                 split: if_splits)
 
 lemma tcbSchedDequeue_tcbSchedNext_tcbSchedPrev_None_obj_at':
@@ -2855,7 +2855,7 @@ lemma (in delete_one_conc_pre) finaliseCap_replaceable:
   apply (frule cte_wp_at_valid_objs_valid_cap', clarsimp+)
   apply (case_tac "cteCap cte",
          simp_all add: isCap_simps capRange_def cap_has_cleanup'_def
-                       final_matters'_def objBits_simps
+                       final_matters'_def gen_objBits_simps
                        not_Final_removeable finaliseCap_def,
          simp_all add: removeable'_def)
      (* thread *)
@@ -3144,6 +3144,8 @@ global_interpretation delete_one_conc_pre
   by (unfold_locales, wp)
      (wp cteDeleteOne_tcbDomain_obj_at' cteDeleteOne_typ_at' cteDeleteOne_reply_pred_tcb_at | simp)+
 
+context begin interpretation Arch . (*FIXME: arch-split*)
+
 lemma cteDeleteOne_invs[wp]:
   "\<lbrace>invs'\<rbrace> cteDeleteOne ptr \<lbrace>\<lambda>rv. invs'\<rbrace>"
   apply (simp add: cteDeleteOne_def unless_def
@@ -3167,11 +3169,13 @@ lemma cteDeleteOne_invs[wp]:
     apply (rule conjI)
      subgoal by auto
     subgoal by (auto dest!: isCapDs simp: pred_tcb_at'_def obj_at'_def projectKOs
-                                     ko_wp_at'_def)
+                                           live'_def hyp_live'_def ko_wp_at'_def)
    apply (wp isFinalCapability_inv getCTE_wp' hoare_weak_lift_imp
         | wp (once) isFinal[where x=ptr])+
   apply (fastforce simp: cte_wp_at_ctes_of)
   done
+
+end
 
 global_interpretation delete_one_conc_fr: delete_one_conc
   by unfold_locales wp
@@ -3255,7 +3259,7 @@ lemma finaliseCap_valid_cap[wp]:
   apply simp
   apply (intro conjI impI)
    apply (clarsimp simp: valid_cap'_def isCap_simps capAligned_def
-                         objBits_simps shiftL_nat)+
+                         gen_objBits_simps shiftL_nat)+
   done
 
 
@@ -3524,7 +3528,7 @@ lemma finaliseCap_corres:
        apply (rule corres_guard_imp)
          apply (rule corres_split[OF unbindMaybeNotification_corres])
            apply (rule cancelAllSignals_corres)
-          apply (wp abs_typ_at_lifts unbind_maybe_notification_invs typ_at_lifts hoare_drop_imps hoare_vcg_all_lift | wpc)+
+          apply (wp abs_typ_at_lifts unbind_maybe_notification_invs gen_typ_at_lifts hoare_drop_imps hoare_vcg_all_lift | wpc)+
         apply (clarsimp simp: valid_cap_def)
        apply (clarsimp simp: valid_cap'_def)
       apply (fastforce simp: final_matters'_def shiftL_nat zbits_map_def)
